IMP-/IMP_Minus_Com.thy
@@ -4,7 +4,7 @@ section "IMP- An even more reduced imperative language"
 
 theory IMP_Minus_Com
   imports
-    Main
+    IMP_Minus_Base
     "HOL-Library.Char_ord"
     "HOL-Library.List_Lexorder"
 begin
@@ -14,32 +14,6 @@ text\<open>Syntax definition for IMP-. Based on the syntax definition of IMP. Co
   we get rid of arithmetic expressions. Instead, we can only assign bit values to registers.
   For the IF and WHILE conditions, we add the possibility to specify a list of registers, such that
   the condition is considered True if at least one of the registers is non-zero. \<close>
-
-datatype bit = Zero | One
-
-fun nat_to_bit:: "nat \<Rightarrow> bit" where
-  "nat_to_bit 0 = Zero" |
-  "nat_to_bit _ = One"
-
-lemma bit_neq_zero_iff[simp]: "x \<noteq> Zero \<longleftrightarrow> x = One" by (cases x) auto
-lemma bit_neq_one_iff[simp]: "x \<noteq> One \<longleftrightarrow> x = Zero" by (cases x) auto
-
-lemma nat_to_bit_eq_One_iff: "nat_to_bit x = One \<longleftrightarrow> x > 0"
-  by (cases x) auto
-
-lemma nat_to_bit_eq_One_iff': "One = nat_to_bit x \<longleftrightarrow> x > 0"
-  by (cases x) auto
-
-lemma nat_to_bit_eq_Zero_iff: "nat_to_bit x = Zero \<longleftrightarrow> x = 0"
-  by (cases x) auto
-
-lemma nat_to_bit_eq_Zero_iff': "Zero = nat_to_bit x \<longleftrightarrow> x = 0"
-  by (cases x) auto
-
-lemmas nat_to_bit_cases = nat_to_bit_eq_One_iff nat_to_bit_eq_One_iff' nat_to_bit_eq_Zero_iff
-  nat_to_bit_eq_Zero_iff'
-
-type_synonym vname = string
 
 datatype
   com = SKIP
