IMP/AExp.thy
@@ -1,10 +1,9 @@
 \<^marker>\<open>creator Bilel Ghorbel, Florian Kessler\<close>
+\<^marker>\<open>creator Fabian Huch\<close>
 theory AExp
   imports
-    Main
-    "HOL-Library.Char_ord"
-    "HOL-Library.List_Lexorder"
-    "HOL-Library.Product_Lexorder"
+    IMP_Base Eq_On
+    "HOL-Library.Char_ord" "HOL-Library.List_Lexorder" "HOL-Library.Product_Lexorder"
 begin
 
 section "Arithmetic Expressions"
@@ -12,18 +11,15 @@ section "Arithmetic Expressions"
 text \<open>We define non-nested arithmetic expressions on natural numbers.
 The defined operations are addition and modified subtraction. Based on the AExp theory of IMP.\<close>
 
-type_synonym vname = string
-type_synonym val = nat
-type_synonym state = "vname \<Rightarrow> val"
+subsection "Atomic expressions:"
 
-text "Defining atomic expressions:"
 datatype atomExp = N val | V vname
 
 fun atomVal :: "atomExp \<Rightarrow> state \<Rightarrow> val" where
   "atomVal (V var) s = s var"|
   "atomVal (N number) _ = number"
 
-text "Defining arithmetic operators and general form of expressions: "
+subsection "Arithmetic operators and general form of expressions: "
 
 datatype aexp = A atomExp | Plus atomExp atomExp | Sub atomExp atomExp
 
@@ -38,35 +34,20 @@ fun aval :: "aexp \<Rightarrow> state \<Rightarrow> val" where
   "aval (a \<oplus> b) s = atomVal a s  + atomVal b s" |
   "aval (a \<ominus> b) s = atomVal a s - atomVal b s"
 
-text "Syntactic sugar to write states:"
-definition null_state ("<>") where
-  "null_state \<equiv> \<lambda>x. 0"
-syntax
-  "_State" :: "updbinds => 'a" ("<_>")
-translations
-  "_State ms" == "_Update <> ms"
-  "_State (_updbinds b bs)" <= "_Update (_State b) bs"
 
-bundle state_syntax
-begin
-notation null_state ("<>")
-end
+section "Instances"
+
+subsection "Atomic expressions"
 
 instantiation atomExp :: order_bot
 begin
-
 fun less_eq_atomExp :: "atomExp \<Rightarrow> atomExp \<Rightarrow> bool" where
   "less_eq_atomExp (N n1) (N n2) \<longleftrightarrow> n1 \<le> n2"
 | "less_eq_atomExp (V v1) (V v2) \<longleftrightarrow> v1 \<le> v2"
 | "less_eq_atomExp (N _) _ \<longleftrightarrow> True"
 | "less_eq_atomExp (V _) _ \<longleftrightarrow> False"
-
-definition less_atomExp :: "atomExp \<Rightarrow> atomExp \<Rightarrow> bool" where
-  "less_atomExp c1 c2 = (c1 \<le> c2 \<and> \<not> c2 \<le> c1)"
-
-definition bot_atomExp :: "atomExp" where
-  "bot_atomExp = N 0"
-
+definition less_atomExp :: "atomExp \<Rightarrow> atomExp \<Rightarrow> bool" where "less_atomExp c1 c2 = (c1 \<le> c2 \<and> \<not> c2 \<le> c1)"
+definition bot_atomExp :: "atomExp" where "bot_atomExp = N 0"
 instance
 proof(standard, goal_cases)
   case 1 show ?case by (simp add: less_atomExp_def)
@@ -81,9 +62,40 @@ next
 qed
 end
 
+instantiation atomExp :: vars
+begin
+fun vars_atomExp :: "atomExp \<Rightarrow> vname list" where
+"vars_atomExp (V var) = [var]" |
+"vars_atomExp (N _) = []"
+instance ..
+end
+
+instantiation atomExp :: subst
+begin
+fun subst_atomExp :: "(vname \<Rightarrow> vname) \<Rightarrow> atomExp \<Rightarrow> atomExp" where
+"subst m (V var) = V (m var)" |
+"subst m (N n) = N n"
+instance
+proof (standard, goal_cases)
+  case (1 m c)
+  then show ?case by (induction c) auto
+qed
+end
+
+instantiation atomExp :: max_const
+begin
+fun max_const_atomExp :: "atomExp \<Rightarrow> nat" where
+"max_const (V _) = 0" |
+"max_const (N n) = n"
+instance ..
+end
+
+
+
+subsection "Arithmetic expressions"
+
 instantiation aexp :: order_bot
 begin
-
 fun less_eq_aexp :: "aexp \<Rightarrow> aexp \<Rightarrow> bool" where
   "less_eq_aexp (A a1) (A a2) \<longleftrightarrow> a1 \<le> a2"
 | "less_eq_aexp (Plus a1 a2) (Plus b1 b2) \<longleftrightarrow> (a1, a2) \<le> (b1, b2)"
@@ -92,13 +104,8 @@ fun less_eq_aexp :: "aexp \<Rightarrow> aexp \<Rightarrow> bool" where
 | "less_eq_aexp _ (A _) \<longleftrightarrow> False"
 | "less_eq_aexp (Plus _ _) _ \<longleftrightarrow> True"
 | "less_eq_aexp _ (Plus _ _) \<longleftrightarrow> False"
-
-definition less_aexp :: "aexp \<Rightarrow> aexp \<Rightarrow> bool" where
-  "less_aexp c1 c2 = (c1 \<le> c2 \<and> \<not> c2 \<le> c1)"
-
-definition bot_aexp :: "aexp" where
-  "bot_aexp = A bot"
-
+definition less_aexp :: "aexp \<Rightarrow> aexp \<Rightarrow> bool" where "less_aexp c1 c2 = (c1 \<le> c2 \<and> \<not> c2 \<le> c1)"
+definition bot_aexp :: "aexp" where "bot_aexp = A bot"
 instance
 proof(standard, goal_cases)
   case 1 show ?case by (simp add: less_aexp_def)
@@ -109,9 +116,99 @@ next
 next
   case (4 x y) thus ?case by (cases x; cases y) auto
 next
-  case 5 show ?case
-    unfolding bot_aexp_def using bot_atomExp_def less_eq_aexp.elims(3) by fastforce
+  case 5 show ?case unfolding bot_aexp_def using bot_atomExp_def less_eq_aexp.elims(3) by fastforce
 qed
 end
+
+instantiation aexp :: vars
+begin
+fun vars_aexp :: "aexp \<Rightarrow> vname list" where
+"vars (A e) = vars e" |
+"vars (Plus e\<^sub>1 e\<^sub>2) = vars e\<^sub>1 @ vars e\<^sub>2" |
+"vars (Sub e\<^sub>1 e\<^sub>2) = vars e\<^sub>1 @ vars e\<^sub>2"
+instance ..
+end
+
+instantiation aexp :: subst
+begin
+fun subst_aexp :: "(vname \<Rightarrow> vname) \<Rightarrow> aexp \<Rightarrow> aexp" where
+"subst m (A e) = A (subst m e)" |
+"subst m (Plus e\<^sub>1 e\<^sub>2) = Plus (subst m e\<^sub>1) (subst m e\<^sub>2)" |
+"subst m (Sub e\<^sub>1 e\<^sub>2) = Sub (subst m e\<^sub>1) (subst m e\<^sub>2)"
+instance
+proof (standard, goal_cases)
+  case (1 m c)
+  then show ?case by (induction c) auto
+qed
+end
+
+instantiation aexp :: max_const
+begin
+fun max_const_aexp :: "aexp \<Rightarrow> nat" where
+"max_const (A e) = max_const e" |
+"max_const (Plus e\<^sub>1 e\<^sub>2) = max (max_const e\<^sub>1) (max_const e\<^sub>2)" |
+"max_const (Sub e\<^sub>1 e\<^sub>2) = max (max_const e\<^sub>1) (max_const e\<^sub>2)"
+instance ..
+end
+
+
+
+section "Facts"
+
+lemma atomVal_eq_if_eq_on_vars[simp]:
+  "s\<^sub>1 = s\<^sub>2 on set (vars a) \<Longrightarrow> atomVal a s\<^sub>1 = atomVal a s\<^sub>2"
+  by (induction a) auto
+
+lemma aval_eq_if_eq_on_vars [simp]:
+  "s\<^sub>1 = s\<^sub>2 on set (vars a) \<Longrightarrow> aval a s\<^sub>1 = aval a s\<^sub>2"
+  apply (induction a)
+  apply auto
+  using atomVal_eq_if_eq_on_vars eq_on_subset
+  apply (metis sup.cobounded1 sup.cobounded2)+
+  done
+
+lemma atomVal_subst[simp]: "inj_on m (set (vars a)) \<Longrightarrow> atomVal (subst m a) s = (atomVal a (s o m))"
+  by (induction a) auto
+
+lemma aval_subst[simp]: "inj_on m (set (vars a)) \<Longrightarrow> aval (subst m a) s = aval a (s o m)"
+  by (induction a) (auto simp add: inj_on_Un)
+
+
+lemma Max_range_le_then_element_le: "finite (range s) \<Longrightarrow> 2 * Max (range s) < (x :: nat) \<Longrightarrow> 2 * (s y) < x"
+proof -
+  assume "2 * Max (range s) < (x :: nat)"
+  moreover have "s y \<in> range s" by simp
+  moreover assume "finite (range s)"
+  moreover hence "s y \<le> Max (range s)" by simp
+  ultimately show ?thesis by linarith
+qed
+
+lemma aval_le_when:
+  assumes "finite (range s)" "2 * max (Max (range s)) (max_const a) < x"
+  shows "aval a s < x"
+using assms proof(cases a)
+  case (A x1)
+  thus ?thesis using assms
+  proof(cases x1)
+    case (V x2)
+    thus ?thesis using assms A Max_range_le_then_element_le[where ?s=s and ?x = x and ?y=x2] by simp
+  qed simp
+next
+  case (Plus x21 x22)
+  hence "2 * max (AExp.atomVal x21 s) (AExp.atomVal x22 s) < x"
+    apply(cases x21; cases x22)
+    using assms
+    by (auto simp add: Max_range_le_then_element_le nat_mult_max_right)
+  thus ?thesis using Plus by auto
+next
+  case (Sub x31 x32)
+  then show ?thesis
+    apply(cases x31 ; cases x32)
+    using assms apply(auto simp add: Max_range_le_then_element_le nat_mult_max_right)
+    using Max_range_le_then_element_le
+    by (metis gr_implies_not0 lessI less_imp_diff_less less_imp_le_nat less_le_trans
+        linorder_neqE_nat n_less_m_mult_n numeral_2_eq_2)+
+qed
+
 
 end
