IMP/Com.thy
@@ -1,12 +1,7 @@
 \<^marker>\<open>creator Bilel Ghorbel, Florian Kessler\<close>
 section "IMP A reduced imperative language"
 theory Com
-  imports
-    Main
-    AExp
-    "HOL-Library.Char_ord"
-    "HOL-Library.List_Lexorder"
-    "HOL-Library.Product_Lexorder"
+  imports AExp
 begin
 
 paragraph "Summary"
@@ -25,6 +20,9 @@ and Seq ("_;;/ _"  [60, 61] 60)
 and If ("(IF _/\<noteq>0 THEN _/ ELSE _)"  [0, 0, 61] 61)
 and While ("(WHILE _/\<noteq>0 DO _)"  [0, 61] 61)
 end
+
+
+section "Instances"
 
 instantiation com :: order_bot
 begin
@@ -65,5 +63,63 @@ next
     unfolding bot_com_def by simp
 qed
 end
+
+instantiation com :: vars
+begin
+fun vars_com :: "com \<Rightarrow> vname list" where
+"vars SKIP = []" |
+"vars (x::=e) = x#vars e" |
+"vars (c1;;c2) = vars c1 @ vars c2" |
+"vars (IF b\<noteq>0 THEN c1 ELSE c2) = b # vars c1 @ vars c2" |
+"vars (WHILE b\<noteq>0 DO c) = b#vars c"
+instance ..
+end
+
+instantiation com :: subst
+begin
+fun subst_com :: "(vname \<Rightarrow> vname) \<Rightarrow> com \<Rightarrow> com" where
+"subst m SKIP = SKIP" |
+"subst m (x::=e) = (m x) ::= subst m e" |
+"subst m (c\<^sub>1;;c\<^sub>2) = subst m c\<^sub>1;; subst m c\<^sub>2" |
+"subst m (IF b\<noteq>0 THEN c\<^sub>1 ELSE c\<^sub>2) = IF m b\<noteq>0 THEN subst m c\<^sub>1 ELSE subst m c\<^sub>2" |
+"subst m (WHILE b\<noteq>0 DO c) = WHILE m b\<noteq>0 DO subst m c"
+instance
+proof (standard, goal_cases)
+  case (1 m c)
+  then show ?case by (induction c) auto
+qed
+end
+
+instantiation com :: max_const
+begin
+fun max_const_com :: "com \<Rightarrow> nat" where
+"max_const SKIP = 0" |
+"max_const (_ ::= e) = max_const e" |
+"max_const (c1;;c2) = max (max_const c1) (max_const c2)" |
+"max_const (IF _\<noteq>0 THEN c1 ELSE c2) = max (max_const c1) (max_const c2)" |
+"max_const (WHILE _\<noteq>0 DO c) = max_const c"
+instance ..
+end
+
+
+section "More Definitions and Facts"
+
+lemma subset_then_length_remdups_le: "set as \<subseteq> set bs
+  \<Longrightarrow> length (remdups (as @ cs)) \<le> length (remdups (bs @ cs))"
+  apply(induction cs)
+   apply (auto simp: card_mono length_remdups_card_conv)
+  by (metis (no_types, lifting) List.finite_set Un_insert_right card_mono dual_order.trans
+      finite.insertI finite_Un sup.boundedI sup.cobounded1 sup.cobounded2)
+
+definition num_vars:: "com \<Rightarrow> nat" where
+"num_vars c = length (remdups (vars c))"
+
+fun lvars :: "com \<Rightarrow> vname set" where
+"lvars SKIP = {}" |
+"lvars (x::=e) = {x}" |
+"lvars (c1;;c2) = lvars c1 \<union> lvars c2" |
+"lvars (IF b\<noteq>0 THEN c1 ELSE c2) = lvars c1 \<union> lvars c2" |
+"lvars (WHILE b\<noteq>0 DO c) = lvars c"
+
 
 end
