IMP-/IMP_Minus_Base.thy
@@ -1,0 +1,33 @@
+theory IMP_Minus_Base
+  imports Main
+begin
+
+datatype bit = Zero | One
+
+type_synonym vname = string
+
+type_synonym state = "vname \<rightharpoonup> bit"
+
+fun nat_to_bit:: "nat \<Rightarrow> bit" where
+  "nat_to_bit 0 = Zero" |
+  "nat_to_bit _ = One"
+
+lemma bit_neq_zero_iff[simp]: "x \<noteq> Zero \<longleftrightarrow> x = One" by (cases x) auto
+lemma bit_neq_one_iff[simp]: "x \<noteq> One \<longleftrightarrow> x = Zero" by (cases x) auto
+
+lemma nat_to_bit_eq_One_iff: "nat_to_bit x = One \<longleftrightarrow> x > 0"
+  by (cases x) auto
+
+lemma nat_to_bit_eq_One_iff': "One = nat_to_bit x \<longleftrightarrow> x > 0"
+  by (cases x) auto
+
+lemma nat_to_bit_eq_Zero_iff: "nat_to_bit x = Zero \<longleftrightarrow> x = 0"
+  by (cases x) auto
+
+lemma nat_to_bit_eq_Zero_iff': "Zero = nat_to_bit x \<longleftrightarrow> x = 0"
+  by (cases x) auto
+
+lemmas nat_to_bit_cases = nat_to_bit_eq_One_iff nat_to_bit_eq_One_iff' nat_to_bit_eq_Zero_iff
+  nat_to_bit_eq_Zero_iff'
+
+end
