IMP/IMP_Base.thy
@@ -1,0 +1,38 @@
+\<^marker>\<open>creator Fabian Huch\<close>
+theory IMP_Base
+  imports Main
+begin
+
+type_synonym vname = string
+type_synonym val = nat
+type_synonym state = "vname \<Rightarrow> val"
+
+text "Syntactic sugar to write states:"
+definition null_state ("<>") where
+  "null_state \<equiv> \<lambda>x. 0"
+syntax
+  "_State" :: "updbinds => 'a" ("<_>")
+translations
+  "_State ms" == "_Update <> ms"
+  "_State (_updbinds b bs)" <= "_Update (_State b) bs"
+
+bundle state_syntax
+begin
+notation null_state ("<>")
+end
+
+section \<open>Important operations\<close>
+
+text \<open>Variables, syntactic substitution, and maximum constant\<close>
+
+class vars =
+  fixes vars :: "'a \<Rightarrow> vname list"
+
+class subst = vars +
+  fixes subst :: "(vname \<Rightarrow> vname) \<Rightarrow> 'a \<Rightarrow> 'a"
+  assumes subst_vars[simp]: "set (vars (subst m c)) = m ` set (vars c)"
+
+class max_const =
+  fixes max_const :: "'a \<Rightarrow> nat"
+
+end
